
\documentclass[pdf]{beamer} 
\mode<presentation>{\usetheme{Madrid}}

\input{packages_beamer.tex}

\title{$A=LU$}
\subtitle{}
\author{}


\begin{document}

\begin{frame}{}
\begin{center}LU Decomposition, Partial pivoting\end{center} $$A = \begin{pmatrix}1&2&4\\1&0&1\\-2&2&4\end{pmatrix}$$\end{frame}
\begin{frame}{}\begin{align*} k &= {\color{red}1} & p({\color{blue}3}) &= 3\end{align*} $$P_{\text{new}}A=\begin{pmatrix}1&0&0\\0&1&0\\0&0&1\end{pmatrix} P_{\text{new}} \begin{pmatrix}1&2&4\\1&0&1\\\boxed{-2}&2&4\end{pmatrix} \quad\quad \begin{pmatrix}1&2&4\\1&0&1\\-2&2&4\end{pmatrix}$$ \begin{align*} p&= \begin{Bmatrix}1&2&3\end{Bmatrix} & P&= \begin{pmatrix}1&0&0\\0&1&0\\0&0&1\end{pmatrix}\\ p_{\text{new}} &= \mathsf{swap}_{{\color{red}1},{\color{blue}3}} \circ \begin{Bmatrix}1&2&3\end{Bmatrix} & P_{\text{new}} &= \begin{pmatrix}0&0&{\color{purple}1}\\0&1&0\\{\color{purple}1}&0&0\end{pmatrix} \begin{pmatrix}1&0&0\\0&1&0\\0&0&1\end{pmatrix}\\ &=\begin{Bmatrix}3&2&1\end{Bmatrix} &&=\begin{pmatrix}0&0&1\\0&1&0\\1&0&0\end{pmatrix}\end{align*}\end{frame}
\begin{frame}{}\begin{align*} k &= 1 & i &= 2 & p(1) &= 3 & p(2) &= 2\end{align*} $$PA=\begin{pmatrix}1&0&0\\0&1&0\\0&0&1\end{pmatrix} P \boxed{\begin{pmatrix}1&2&4\\\mathbf{{\color{blue}1}}&\mathbf{0}&\mathbf{1}\\\boxed{{\color{red}-2}}&2&4\end{pmatrix}} \quad\quad \begin{pmatrix}1&2&4\\{\color{purple}-0.5}&1&3\\-2&2&4\end{pmatrix}$$ \begin{align*} p&= \begin{Bmatrix}3&2&1\end{Bmatrix} & P&= \begin{pmatrix}0&0&1\\0&1&0\\1&0&0\end{pmatrix} \end{align*} $$R_{p(2)} \mapsfrom R_{p(2)} - \frac{{\color{blue}1}}{{\color{red}-2}} R_{p(1)}$$ $$ \begin{pmatrix}1&0&0\\{\color{red}0.5}&1&0\\0&0&1\end{pmatrix} P \boxed{\begin{pmatrix}1&2&4\\\mathbf{1}&\mathbf{0}&\mathbf{1}\\-2&2&4\end{pmatrix}} = P \begin{pmatrix}1&2&4\\\mathbf{0}&\mathbf{1}&\mathbf{3}\\-2&2&4\end{pmatrix} $$\end{frame}
\begin{frame}{}\begin{align*} k &= 1 & i &= 2 & p(1) &= 3 & p(2) &= 2\end{align*} $$PA=\begin{pmatrix}1&0&0\\0&1&0\\0&0&1\end{pmatrix} P \boxed{\begin{pmatrix}1&2&4\\\mathbf{{\color{blue}1}}&\mathbf{0}&\mathbf{1}\\\boxed{{\color{red}-2}}&2&4\end{pmatrix}} \quad\quad \begin{pmatrix}1&2&4\\{\color{purple}-0.5}&1&3\\-2&2&4\end{pmatrix}$$ \begin{align*} p&= \begin{Bmatrix}3&2&1\end{Bmatrix} & P&= \begin{pmatrix}0&0&1\\0&1&0\\1&0&0\end{pmatrix} \end{align*} $$R_{p(2)} \mapsfrom R_{p(2)} - \frac{{\color{blue}1}}{{\color{red}-2}} R_{p(1)}$$ $$ P \boxed{\begin{pmatrix}1&2&4\\\mathbf{1}&\mathbf{0}&\mathbf{1}\\-2&2&4\end{pmatrix}} = \begin{pmatrix}1&0&0\\{\color{red}-0.5}&1&0\\0&0&1\end{pmatrix} P \begin{pmatrix}1&2&4\\\mathbf{0}&\mathbf{1}&\mathbf{3}\\-2&2&4\end{pmatrix} $$\end{frame}
\begin{frame}{}\begin{align*} k &= 1 & i &= 2 & p(1) &= 3 & p(2) &= 2\end{align*}$$PA=\begin{pmatrix}1&0&0\\{\color{red}-0.5}&1&0\\0&0&1\end{pmatrix} P \begin{pmatrix}1&2&4\\\mathbf{0}&\mathbf{1}&\mathbf{3}\\\boxed{-2}&2&4\end{pmatrix} \quad\quad \begin{pmatrix}1&2&4\\{\color{purple}-0.5}&1&3\\-2&2&4\end{pmatrix}$$\begin{align*} p&= \begin{Bmatrix}3&2&1\end{Bmatrix} & P&= \begin{pmatrix}0&0&1\\0&1&0\\1&0&0\end{pmatrix} \end{align*}\end{frame}
\begin{frame}{}\begin{align*} k &= 1 & i &= 3 & p(1) &= 3 & p(3) &= 1\end{align*} $$PA=\begin{pmatrix}1&0&0\\-0.5&1&0\\0&0&1\end{pmatrix} P \boxed{\begin{pmatrix}\mathbf{{\color{blue}1}}&\mathbf{2}&\mathbf{4}\\0&1&3\\\boxed{{\color{red}-2}}&2&4\end{pmatrix}} \quad\quad \begin{pmatrix}{\color{purple}-0.5}&3&6\\{\color{purple}-0.5}&1&3\\-2&2&4\end{pmatrix}$$ \begin{align*} p&= \begin{Bmatrix}3&2&1\end{Bmatrix} & P&= \begin{pmatrix}0&0&1\\0&1&0\\1&0&0\end{pmatrix} \end{align*} $$R_{p(3)} \mapsfrom R_{p(3)} - \frac{{\color{blue}1}}{{\color{red}-2}} R_{p(1)}$$ $$ \begin{pmatrix}1&0&0\\0&1&0\\{\color{red}0.5}&0&1\end{pmatrix} P \boxed{\begin{pmatrix}\mathbf{1}&\mathbf{2}&\mathbf{4}\\0&1&3\\-2&2&4\end{pmatrix}} = P \begin{pmatrix}\mathbf{0}&\mathbf{3}&\mathbf{6}\\0&1&3\\-2&2&4\end{pmatrix} $$\end{frame}
\begin{frame}{}\begin{align*} k &= 1 & i &= 3 & p(1) &= 3 & p(3) &= 1\end{align*} $$PA=\begin{pmatrix}1&0&0\\-0.5&1&0\\0&0&1\end{pmatrix} P \boxed{\begin{pmatrix}\mathbf{{\color{blue}1}}&\mathbf{2}&\mathbf{4}\\0&1&3\\\boxed{{\color{red}-2}}&2&4\end{pmatrix}} \quad\quad \begin{pmatrix}{\color{purple}-0.5}&3&6\\{\color{purple}-0.5}&1&3\\-2&2&4\end{pmatrix}$$ \begin{align*} p&= \begin{Bmatrix}3&2&1\end{Bmatrix} & P&= \begin{pmatrix}0&0&1\\0&1&0\\1&0&0\end{pmatrix} \end{align*} $$R_{p(3)} \mapsfrom R_{p(3)} - \frac{{\color{blue}1}}{{\color{red}-2}} R_{p(1)}$$ $$ P \boxed{\begin{pmatrix}\mathbf{1}&\mathbf{2}&\mathbf{4}\\0&1&3\\-2&2&4\end{pmatrix}} = \begin{pmatrix}1&0&0\\0&1&0\\{\color{red}-0.5}&0&1\end{pmatrix} P \begin{pmatrix}\mathbf{0}&\mathbf{3}&\mathbf{6}\\0&1&3\\-2&2&4\end{pmatrix} $$\end{frame}
\begin{frame}{}\begin{align*} k &= 1 & i &= 3 & p(1) &= 3 & p(3) &= 1\end{align*}$$PA=\begin{pmatrix}1&0&0\\-0.5&1&0\\{\color{red}-0.5}&0&1\end{pmatrix} P \begin{pmatrix}\mathbf{0}&\mathbf{3}&\mathbf{6}\\0&1&3\\\boxed{-2}&2&4\end{pmatrix} \quad\quad \begin{pmatrix}{\color{purple}-0.5}&3&6\\{\color{purple}-0.5}&1&3\\-2&2&4\end{pmatrix}$$\begin{align*} p&= \begin{Bmatrix}3&2&1\end{Bmatrix} & P&= \begin{pmatrix}0&0&1\\0&1&0\\1&0&0\end{pmatrix} \end{align*}\end{frame}
\begin{frame}{}\begin{align*} k &= {\color{red}2} & p({\color{blue}3}) &= 1\end{align*} $$P_{\text{new}}A=\begin{pmatrix}1&0&0\\{\color{purple}-0.5}&1&0\\{\color{purple}-0.5}&0&1\end{pmatrix} P_{\text{new}} \begin{pmatrix}0&\boxed{3}&6\\0&1&3\\-2&2&4\end{pmatrix} \quad\quad \begin{pmatrix}{\color{purple}-0.5}&3&6\\{\color{purple}-0.5}&1&3\\-2&2&4\end{pmatrix}$$ \begin{align*} p&= \begin{Bmatrix}3&2&1\end{Bmatrix} & P&= \begin{pmatrix}0&0&1\\0&1&0\\1&0&0\end{pmatrix}\\ p_{\text{new}} &= \mathsf{swap}_{{\color{red}2},{\color{blue}3}} \circ \begin{Bmatrix}3&2&1\end{Bmatrix} & P_{\text{new}} &= \begin{pmatrix}1&0&0\\0&0&{\color{purple}1}\\0&{\color{purple}1}&0\end{pmatrix} \begin{pmatrix}0&0&1\\0&1&0\\1&0&0\end{pmatrix}\\ &=\begin{Bmatrix}3&1&2\end{Bmatrix} &&=\begin{pmatrix}0&0&1\\1&0&0\\0&1&0\end{pmatrix}\end{align*}\end{frame}
\begin{frame}{}\begin{align*} k &= 2 & i &= 3 & p(2) &= 1 & p(3) &= 2\end{align*} $$PA=\begin{pmatrix}1&0&0\\-0.5&1&0\\-0.5&0&1\end{pmatrix} P \boxed{\begin{pmatrix}0&\boxed{{\color{red}3}}&6\\\mathbf{0}&\mathbf{{\color{blue}1}}&\mathbf{3}\\-2&2&4\end{pmatrix}} \quad\quad \begin{pmatrix}{\color{purple}-0.5}&3&6\\{\color{purple}-0.5}&{\color{purple}0.333333}&1\\-2&2&4\end{pmatrix}$$ \begin{align*} p&= \begin{Bmatrix}3&1&2\end{Bmatrix} & P&= \begin{pmatrix}0&0&1\\1&0&0\\0&1&0\end{pmatrix} \end{align*} $$R_{p(3)} \mapsfrom R_{p(3)} - \frac{{\color{blue}1}}{{\color{red}3}} R_{p(2)}$$ $$ \begin{pmatrix}1&0&0\\0&1&0\\0&{\color{red}-0.333333}&1\end{pmatrix} P \boxed{\begin{pmatrix}0&3&6\\\mathbf{0}&\mathbf{1}&\mathbf{3}\\-2&2&4\end{pmatrix}} = P \begin{pmatrix}0&3&6\\\mathbf{0}&\mathbf{0}&\mathbf{1}\\-2&2&4\end{pmatrix} $$\end{frame}
\begin{frame}{}\begin{align*} k &= 2 & i &= 3 & p(2) &= 1 & p(3) &= 2\end{align*} $$PA=\begin{pmatrix}1&0&0\\-0.5&1&0\\-0.5&0&1\end{pmatrix} P \boxed{\begin{pmatrix}0&\boxed{{\color{red}3}}&6\\\mathbf{0}&\mathbf{{\color{blue}1}}&\mathbf{3}\\-2&2&4\end{pmatrix}} \quad\quad \begin{pmatrix}{\color{purple}-0.5}&3&6\\{\color{purple}-0.5}&{\color{purple}0.333333}&1\\-2&2&4\end{pmatrix}$$ \begin{align*} p&= \begin{Bmatrix}3&1&2\end{Bmatrix} & P&= \begin{pmatrix}0&0&1\\1&0&0\\0&1&0\end{pmatrix} \end{align*} $$R_{p(3)} \mapsfrom R_{p(3)} - \frac{{\color{blue}1}}{{\color{red}3}} R_{p(2)}$$ $$ P \boxed{\begin{pmatrix}0&3&6\\\mathbf{0}&\mathbf{1}&\mathbf{3}\\-2&2&4\end{pmatrix}} = \begin{pmatrix}1&0&0\\0&1&0\\0&{\color{red}0.333333}&1\end{pmatrix} P \begin{pmatrix}0&3&6\\\mathbf{0}&\mathbf{0}&\mathbf{1}\\-2&2&4\end{pmatrix} $$\end{frame}
\begin{frame}{}\begin{align*} k &= 2 & i &= 3 & p(2) &= 1 & p(3) &= 2\end{align*}$$PA=\begin{pmatrix}1&0&0\\-0.5&1&0\\-0.5&{\color{red}0.333333}&1\end{pmatrix} P \begin{pmatrix}0&\boxed{3}&6\\\mathbf{0}&\mathbf{0}&\mathbf{1}\\-2&2&4\end{pmatrix} \quad\quad \begin{pmatrix}{\color{purple}-0.5}&3&6\\{\color{purple}-0.5}&{\color{purple}0.333333}&1\\-2&2&4\end{pmatrix}$$\begin{align*} p&= \begin{Bmatrix}3&1&2\end{Bmatrix} & P&= \begin{pmatrix}0&0&1\\1&0&0\\0&1&0\end{pmatrix} \end{align*}\end{frame}
\begin{frame}{}\begin{align*}PA&=\begin{pmatrix}1&0&0\\-0.5&1&0\\-0.5&0.333333&1\end{pmatrix} P \begin{pmatrix}0&3&6\\0&0&1\\-2&2&4\end{pmatrix}\\&= \begin{pmatrix}1&0&0\\-0.5&1&0\\-0.5&0.333333&1\end{pmatrix} \begin{pmatrix}-2&2&4\\0&3&6\\0&0&1\end{pmatrix} \\ P&= \begin{pmatrix}0&0&1\\1&0&0\\0&1&0\end{pmatrix}\end{align*}
\end{frame}

\end{document}
